

# 1 Goal

The goal is to optimize the following:

$$\begin{aligned} \min_{\boldsymbol{\beta}} \quad & \sum_{i=1}^n \mathbf{PLQ}(y_i, \mathbf{x}_i^\top \boldsymbol{\beta}) + \frac{1}{2} \|\boldsymbol{\beta}\|_2^2 + \rho \|\boldsymbol{\beta}\|_1 \\ \text{s. t. } & \mathbf{A}\boldsymbol{\beta} + \mathbf{b} \geq \mathbf{0} \end{aligned}$$

After ReLU-ReHU decomposition on the PLQ loss:

$$\begin{aligned} \min_{\boldsymbol{\beta}} \quad & \sum_{l,i} \mathbf{ReLU}(u_{li} \mathbf{x}_i^\top \boldsymbol{\beta} + v_{li}) + \sum_{h,i} \mathbf{ReHU}_{\tau_{hi}}(s_{hi} \mathbf{x}_i^\top \boldsymbol{\beta} + t_{hi}) + \frac{1}{2} \|\boldsymbol{\beta}\|_2^2 + \rho \sum_{j=1}^d |\beta_j| \\ \text{s. t. } & \mathbf{A}\boldsymbol{\beta} + \mathbf{b} \geq \mathbf{0} \\ \Leftrightarrow \quad & \min_{\boldsymbol{\beta}, \Pi, \Sigma, \Theta} \sum_{l,i} \pi_{li} + \sum_{h,i} \frac{1}{2} \theta_{hi}^2 + \sum_{h,i} \tau_{hi} \sigma_{hi} + \frac{1}{2} \|\boldsymbol{\beta}\|_2^2 + \rho \sum_{j=1}^d |\beta_j| \\ \text{s. t. } & \mathbf{A}\boldsymbol{\beta} + \mathbf{b} \geq \mathbf{0}, \quad \pi_{li} - u_{li} \mathbf{x}_i^\top \boldsymbol{\beta} - v_{li} \geq 0, \\ & \theta_{hi} + \sigma_{hi} - s_{hi} \mathbf{x}_i^\top \boldsymbol{\beta} - t_{hi} \geq 0, \\ & \pi_{li} \geq 0, \quad \theta_{hi} \geq 0 \end{aligned}$$

Then we substitute  $\ell_1$  norm terms:

$$\begin{aligned} \min_{\boldsymbol{\beta}, \Pi, \Sigma, \Theta} \quad & \sum_{l,i} \pi_{li} + \sum_{h,i} \frac{1}{2} \theta_{hi}^2 + \sum_{h,i} \tau_{hi} \sigma_{hi} + \frac{1}{2} \|\boldsymbol{\beta}\|_2^2 + \rho \sum_{j=1}^d \omega_j \\ \text{s. t. } & \mathbf{a}_k^\top \boldsymbol{\beta} + b_k \geq 0, \\ & \pi_{li} - u_{li} \mathbf{x}_i^\top \boldsymbol{\beta} - v_{li} \geq 0, \\ & \theta_{hi} + \sigma_{hi} - s_{hi} \mathbf{x}_i^\top \boldsymbol{\beta} - t_{hi} \geq 0, \\ & \pi_{li} \geq 0, \\ & \theta_{hi} \geq 0, \\ & \omega_j - \beta_j \geq 0, \\ & \omega_j + \beta_j \geq 0. \end{aligned}$$

## 2 Prime Problem

$$\begin{aligned}
\mathcal{L}_P = & \sum_{l,i} \pi_{li} + \sum_{h,i} \frac{1}{2} \theta_{hi}^2 + \sum_{h,i} \tau_{hi} \sigma_{hi} + \frac{1}{2} \|\boldsymbol{\beta}\|_2^2 + \rho \sum_{j=1}^d \omega_j \\
& - \sum_k \xi_k \mathbf{a}_k^\top \boldsymbol{\beta} + \sum_k \xi_k b_k - \sum_{l,i} \lambda_{l,i} (\pi_{li} - u_{li} \mathbf{x}_i^\top \boldsymbol{\beta} - v_{li}) \\
& - \sum_{h,i} \gamma_{hi} (\theta_{hi} + \sigma_{hi} - s_{hi} \mathbf{x}_i^\top \boldsymbol{\beta} - t_{hi}) \\
& - \sum_{l,i} \delta_{li} \pi_{li} - \sum_{h,i} \psi_{hi} \sigma_{hi} \\
& - \sum_{j=1}^d \eta_j (\omega_j - \beta_j) - \sum_{j=1}^d \mu_j (\omega_j + \beta_j)
\end{aligned}$$

**KKT Condition gives:**

$$\begin{aligned}
\theta_{hi} &= \gamma_{hi} \\
\delta_{li} &= 1 - \lambda_{li} \\
\psi_{hi} &= \tau_{hi} - \gamma_{hi} \\
\eta_j &= \rho - \mu_j \\
\boldsymbol{\beta} &= \sum_{k=1}^K \xi_k \mathbf{a}_k - \sum_{i=1}^n \mathbf{x}_i \left( \sum_{l=1}^L \lambda_{li} u_{li} + \sum_{h=1}^H \gamma_{hi} s_{hi} \right) + 2\boldsymbol{\mu} - \rho \mathbf{1}_d \\
\beta_j &= \sum_{k=1}^K \xi_k a_{kj} - \sum_{i=1}^n x_{ij} \left( \sum_{l=1}^L \lambda_{li} u_{li} + \sum_{h=1}^H \gamma_{hi} s_{hi} \right) + 2\mu_j - \rho
\end{aligned}$$

### 3 Negative Dual Problem

$$\begin{aligned}
\mathcal{L}_D = & \frac{1}{2} \left( \sum_{k=1}^K \sum_{k'=1}^K \xi_k \xi_{k'} \mathbf{a}_k^\top \mathbf{a}_{k'} + \sum_{l,i} \sum_{l',i'} \lambda_{li} \lambda_{l'i'} u_{li'} u_{l'i} \mathbf{x}_i^\top \mathbf{x}_{i'} + \sum_{h,i} \sum_{h',i'} \gamma_{hi} \gamma_{h'i'} s_{hi} s_{h'i'} \mathbf{x}_i^\top \mathbf{x}_{i'} \right) \\
& - \sum_{k=1}^K \sum_{l,i} \xi_k \lambda_{li} u_{li} \mathbf{a}_k^\top \mathbf{x}_i - \sum_{k=1}^K \sum_{h,i} \xi_k \gamma_{hi} s_{hi} \mathbf{a}_k^\top \mathbf{x}_i + \sum_{l,i} \sum_{h',i'} \lambda_{li} u_{li} \gamma_{h'i'} s_{h'i'} \mathbf{x}_i^\top \mathbf{x}_{i'} \\
& + \frac{1}{2} \sum_{h,i} \gamma_{hi}^2 + \sum_{k=1}^K \xi_k b_k - \sum_{l,i} \lambda_{li} v_{li} - \sum_{h,i} \gamma_{hi} t_{hi} \\
& + \sum_{k=1}^K \xi_k (2\boldsymbol{\mu} - \rho \mathbf{1}_d)^\top \mathbf{a}_k + \sum_{l,i} \lambda_{li} u_{li} (\rho \mathbf{1}_d - 2\boldsymbol{\mu})^\top \mathbf{x}_i + \sum_{h,i} \gamma_{hi} s_{hi} (\rho \mathbf{1}_d - 2\boldsymbol{\mu})^\top \mathbf{x}_i \\
& + 2\boldsymbol{\mu}^\top \boldsymbol{\mu} - 2\boldsymbol{\mu}^\top \rho \mathbf{1}_d + \frac{d\rho^2}{2}
\end{aligned}$$

$$\begin{aligned}
\text{s. t. } & \xi_k \geq 0, \\
& 0 \leq \lambda_{li} \leq 1, \\
& 0 \leq \gamma_{hi} \leq \tau_{hi}, \\
& 0 \leq \mu_d \leq \rho.
\end{aligned}$$

Update  $\mu_j$  and  $\beta_j$  with all other variables fixed:

$$\begin{aligned}
& \min_{\mu_j} \sum_{k=1}^K \xi_k a_{kj} \mu_j - \sum_{i=1}^n \sum_{l=1}^L \lambda_{li} u_{li} x_{ij} \mu_j - \sum_{i=1}^n \sum_{h=1}^H \gamma_{hi} s_{hi} x_{ij} \mu_j + \mu_j^2 - \rho \mu_j \\
\iff & \min_{\mu_j} \mu_j^2 + \left( \sum_{k=1}^K \xi_k a_{kj} - \sum_{i=1}^n \sum_{l=1}^L \lambda_{li} u_{li} x_{ij} - \sum_{i=1}^n \sum_{h=1}^H \gamma_{hi} s_{hi} x_{ij} - \rho \right) \mu_j
\end{aligned}$$

$$\begin{aligned}
\nabla_{\mu_j} \mathcal{L}_D &= 2\mu_j + \sum_{k=1}^K \xi_k a_{kj} - \sum_{i=1}^n \sum_{l=1}^L \lambda_{li} u_{li} x_{ij} - \sum_{i=1}^n \sum_{h=1}^H \gamma_{hi} s_{hi} x_{ij} - \rho \\
&= \beta_j
\end{aligned}$$

$$\begin{aligned}
\mu_j^{\text{new}} &= \mathcal{P}_{[0,\rho]} \left( \mu_j^{\text{old}} - \frac{\beta_j^{\text{old}}}{2} \right) \quad \xLeftrightarrow{\text{parallelize}} \quad \boldsymbol{\mu}^{\text{new}} = \mathcal{P}_{[0,\rho \mathbf{1}]} \left( \boldsymbol{\mu}^{\text{old}} - \frac{\boldsymbol{\beta}^{\text{old}}}{2} \right) \\
\beta_j^{\text{new}} &= \beta_j^{\text{old}} + 2(\mu_j^{\text{new}} - \mu_j^{\text{old}}) \quad \xLeftrightarrow{\text{parallelize}} \quad \boldsymbol{\beta}^{\text{new}} = \boldsymbol{\beta}^{\text{old}} + 2(\boldsymbol{\mu}^{\text{new}} - \boldsymbol{\mu}^{\text{old}})
\end{aligned}$$

**Update  $\xi_k$  and  $\beta$  with all other variables fixed:**

$$\min_{\xi_k} \frac{1}{2} \mathbf{a}_k^\top \mathbf{a}_k \xi_k^2 + \sum_{k' \neq k} \xi_{k'} \mathbf{a}_{k'}^\top \mathbf{a}_k \xi_k - \sum_{l,i} \lambda_{li} u_{li} \xi_k \mathbf{a}_k^\top \mathbf{x}_i - \sum_{h,i} \gamma_{hi} s_{hi} \xi_k \mathbf{a}_k^\top \mathbf{x}_i + b_k \xi_k + (2\boldsymbol{\mu} - \mathbf{1}_d)^\top \mathbf{a}_k \xi_k$$

$$\begin{aligned} \nabla_{\xi_k} \mathcal{L}_{\mathcal{D}} &= \mathbf{a}_k^\top \mathbf{a}_k \xi_k + \sum_{k' \neq k} \xi_{k'} \mathbf{a}_{k'}^\top \mathbf{a}_k - \sum_{l,i} \lambda_{li} u_{li} \mathbf{a}_k^\top \mathbf{x}_i - \sum_{h,i} \gamma_{hi} s_{hi} \mathbf{a}_k^\top \mathbf{x}_i + b_k + (2\boldsymbol{\mu} - \mathbf{1}_d)^\top \mathbf{a}_k \\ &= \sum_{k'=1}^K \xi_{k'} \mathbf{a}_{k'}^\top \mathbf{a}_k - \sum_{l,i} \lambda_{li} u_{li} \mathbf{a}_k^\top \mathbf{x}_i - \sum_{h,i} \gamma_{hi} s_{hi} \mathbf{a}_k^\top \mathbf{x}_i + \mathbf{a}_k^\top (2\boldsymbol{\mu} - \mathbf{1}_d) + b_k \\ &= \mathbf{a}_k^\top \boldsymbol{\beta} + b_k \end{aligned}$$

$$\begin{aligned} \xi_k^{\text{new}} &= \mathcal{P}_{[0,+\infty)} \left( \xi_k^{\text{old}} - \frac{\nabla_{\xi_k} \mathcal{L}(\xi^{\text{old}})}{\|\mathbf{a}_k\|_2^2} \right) = \max \left( 0, \xi_k^{\text{old}} - \frac{\mathbf{a}_k^\top \boldsymbol{\beta}^{\text{old}} + b_k}{\|\mathbf{a}_k\|_2^2} \right) \\ \boldsymbol{\beta}^{\text{new}} &= \boldsymbol{\beta}^{\text{old}} + (\xi_k^{\text{new}} - \xi_k^{\text{old}}) \mathbf{a}_k. \end{aligned}$$

**Update  $\lambda_{li}$  and  $\beta$  with all other variables fixed:**

$$\begin{aligned} \min_{\lambda_{li}} \quad & \frac{1}{2} u_{li}^2 \lambda_{li}^2 \mathbf{x}_i^\top \mathbf{x}_i + \sum_{(l',i') \neq (l,i)} \lambda_{l'i'} u_{l'i'} u_{li} \mathbf{x}_{i'}^\top \mathbf{x}_i \lambda_{li} - \sum_{k=1}^K \xi_k u_{li} \mathbf{a}_k^\top \mathbf{x}_i \lambda_{li} + \sum_{h',i'} u_{li} \gamma_{h'i'} s_{h'i'} \mathbf{x}_{i'}^\top \mathbf{x}_i \lambda_{li} \\ & - v_{li} \lambda_{li} + \lambda_{li} u_{li} (\mathbf{1}_d - 2\boldsymbol{\mu})^\top \mathbf{x}_i \end{aligned}$$

$$\begin{aligned} \nabla_{\lambda_{li}} \mathcal{L}_{\mathcal{D}} &= u_{li}^2 \lambda_{li} \mathbf{x}_i^\top \mathbf{x}_i + \sum_{(l',i') \neq (l,i)} \lambda_{l'i'} u_{l'i'} u_{li} \mathbf{x}_{i'}^\top \mathbf{x}_i - \sum_{k=1}^K \xi_k u_{li} \mathbf{a}_k^\top \mathbf{x}_i + \sum_{h',i'} u_{li} \gamma_{h'i'} s_{h'i'} \mathbf{x}_{i'}^\top \mathbf{x}_i \\ & - v_{li} + u_{li} \mathbf{x}_i^\top (\mathbf{1}_d - 2\boldsymbol{\mu}) \\ & = -u_{li} \mathbf{x}_i^\top \boldsymbol{\beta} - v_{li} \end{aligned}$$

$$\begin{aligned} \lambda_{li}^{\text{new}} &= \mathcal{P}_{[0,1]} \left( \lambda_{li}^{\text{old}} - \frac{\nabla_{\lambda_{li}} \mathcal{L}(\lambda^{\text{old}})}{u_{li}^2 \|\mathbf{x}_i\|_2^2} \right) = \max \left( 0, \min \left( 1, \lambda_{li}^{\text{old}} + \frac{u_{li} \mathbf{x}_i^\top \boldsymbol{\beta}^{\text{old}} + v_{li}}{u_{li}^2 \|\mathbf{x}_i\|_2^2} \right) \right) \\ \boldsymbol{\beta}^{\text{new}} &= \boldsymbol{\beta}^{\text{old}} - (\lambda_{li}^{\text{new}} - \lambda_{li}^{\text{old}}) u_{li} \mathbf{x}_i. \end{aligned}$$

**Update  $\gamma_{hi}$  and  $\beta$  with all other variables fixed:**

$$\begin{aligned} \min_{\gamma_{hi}} \quad & \frac{1}{2}(s_{hi}^2 \mathbf{x}_i^\top \mathbf{x}_i + 1)\gamma_{hi}^2 + \sum_{(h',i') \neq (h,i)} \gamma_{h'i'} s_{h'i'} s_{hi} \mathbf{x}_{i'}^\top \mathbf{x}_i \gamma_{hi} - \sum_{k=1}^K \xi_k s_{hi} \mathbf{a}_k^\top \mathbf{x}_i \gamma_{hi} \\ & + \sum_{l',i'} s_{hi} \lambda_{l'i'} u_{l'i'} \mathbf{x}_i^\top \mathbf{x}_{i'} \gamma_{hi} - t_{hi} \gamma_{hi} + \gamma_{hi} s_{hi} (\mathbf{1}_d - 2\boldsymbol{\mu})^\top \mathbf{x}_i \end{aligned}$$

$$\begin{aligned} \nabla_{\gamma_{hi}} \mathcal{L}_{\mathcal{D}} &= (s_{hi}^2 \mathbf{x}_i^\top \mathbf{x}_i + 1)\gamma_{hi} + \sum_{(h',i') \neq (h,i)} \gamma_{h'i'} s_{h'i'} s_{hi} \mathbf{x}_{i'}^\top \mathbf{x}_i - \sum_{k=1}^K \xi_k s_{hi} \mathbf{a}_k^\top \mathbf{x}_i \\ &\quad + \sum_{l',i'} s_{hi} \lambda_{l'i'} u_{l'i'} \mathbf{x}_i^\top \mathbf{x}_{i'} - t_{hi} + s_{hi} (\mathbf{1}_d - 2\boldsymbol{\mu})^\top \mathbf{x}_i \\ &= \gamma_{hi} + \sum_{h,i} \gamma_{hi} s_{hi} \mathbf{x}_i^\top \mathbf{x}_i - \sum_{k=1}^K \xi_k s_{hi} \mathbf{a}_k^\top \mathbf{x}_i + \sum_{l,i} s_{hi} \lambda_{li} u_{li} \mathbf{x}_i^\top \mathbf{x}_i - t_{hi} \\ &\quad + s_{hi} \mathbf{x}_i^\top (\mathbf{1}_d - 2\boldsymbol{\mu}) \\ &= \gamma_{hi} - s_{hi} \mathbf{x}_i^\top \boldsymbol{\beta} - t_{hi} \end{aligned}$$

$$\begin{aligned} \gamma_{hi}^{\text{new}} &= \mathcal{P}_{[0, \tau_{hi}]} \left( \gamma_{hi}^{\text{old}} - \frac{\nabla_{\gamma_{hi}} \mathcal{L}(\gamma^{\text{old}})}{s_{hi}^2 \|\mathbf{x}_i\|_2^2 + 1} \right) = \max \left( 0, \min \left( \tau_{hi}, \gamma_{hi}^{\text{old}} + \frac{s_{hi} \mathbf{x}_i^\top \boldsymbol{\beta}^{\text{old}} + t_{hi} - \gamma_{hi}^{\text{old}}}{s_{hi}^2 \|\mathbf{x}_i\|_2^2 + 1} \right) \right), \\ \boldsymbol{\beta}^{\text{new}} &= \boldsymbol{\beta}^{\text{old}} - (\gamma_{hi}^{\text{new}} - \gamma_{hi}^{\text{old}}) s_{hi} \mathbf{x}_i. \end{aligned} \tag{B.11}$$